riscv machine+design+crefine: explicitly set pptrTop
Factor out pptrTop from the definition in kernelELFBase and define it
as a constant as on other platforms. Shadows the equivalent definition
in Haskell.

Also remove incorrect comment -- the term was not PADDR_TOP, but
PPTR_TOP in C.

Co-authored-by: Corey Lewis <corey.lewis@proofcraft.systems>
Signed-off-by: Gerwin Klein <gerwin.klein@proofcraft.systems>

spec/machine/RISCV64/Platform.thy
@@ -109,10 +109,13 @@ definition kernelELFPAddrBase :: machine_word
   where
   "kernelELFPAddrBase = physBase + 0x4000000"
 
+definition pptrTop :: machine_word
+  where
+  "pptrTop \<equiv> - (1 << 31)"
+
 definition kernelELFBase :: machine_word
   where
-  (* note: the - (1 << 31) here is PADDR_TOP in C *)
-  "kernelELFBase = - (1 << 31) + (kernelELFPAddrBase && mask 30)" (* 2^64 - 2 GiB + ... *)
+  "kernelELFBase = pptrTop + (kernelELFPAddrBase && mask 30)" (* 2^64 - 2 GiB + ... *)
 
 definition kernelELFBaseOffset :: machine_word
   where
