spec/design/skel/RISCV64/Hardware_H.thy
@@ -12,7 +12,7 @@ begin
 
 context Arch begin global_naming RISCV64_H
 
-#INCLUDE_HASKELL SEL4/Machine/Hardware/RISCV64.hs Platform=Platform.RISCV64 CONTEXT RISCV64_H NOT plic_complete_claim getMemoryRegions getDeviceRegions getKernelDevices loadWord storeWord storeWordVM getActiveIRQ ackInterrupt maskInterrupt configureTimer resetTimer debugPrint getRestartPC setNextPC clearMemory clearMemoryVM initMemory freeMemory setHardwareASID wordFromPDE wordFromPTE VMFaultType HypFaultType VMPageSize pageBits pageBitsForSize toPAddr addrFromPPtr ptrFromPAddr sfence physBase paddrBase pptrBase pptrBaseOffset pptrUserTop kernelELFBase kernelELFBaseOffset kernelELFPAddrBase addrFromKPPtr ptTranslationBits vmFaultTypeFSR read_stval setVSpaceRoot hwASIDFlush setIRQTrigger
+#INCLUDE_HASKELL SEL4/Machine/Hardware/RISCV64.hs Platform=Platform.RISCV64 CONTEXT RISCV64_H NOT plic_complete_claim getMemoryRegions getDeviceRegions getKernelDevices loadWord storeWord storeWordVM getActiveIRQ ackInterrupt maskInterrupt configureTimer resetTimer debugPrint getRestartPC setNextPC clearMemory clearMemoryVM initMemory freeMemory setHardwareASID wordFromPDE wordFromPTE VMFaultType HypFaultType VMPageSize pageBits pageBitsForSize toPAddr addrFromPPtr ptrFromPAddr sfence physBase paddrBase pptrBase pptrBaseOffset pptrTop pptrUserTop kernelELFBase kernelELFBaseOffset kernelELFPAddrBase addrFromKPPtr ptTranslationBits vmFaultTypeFSR read_stval setVSpaceRoot hwASIDFlush setIRQTrigger
 
 end
 
